Dafny/examples/simpleBenign/BenignCode.s.dfy
@@ -1,0 +1,49 @@
+include "../../LLVM/llvmREFACTOR.i.dfy"
+include "../../LLVM/types.dfy"
+include "../../LLVM/control_flow.i.dfy"
+include "../../LLVM/behaviorLemmas.i.dfy"
+include "../../Libraries/Seqs.s.dfy"
+include "../../LLVM/memory.i.dfy"
+
+module challenge6Code{
+    import opened control_flow
+    import opened LLVM_defRE
+    import opened types
+    import opened Collections__Seqs_s
+    import opened behavior_lemmas
+    import opened memory
+
+
+    function challenge_7_transport_handler_code():codeRe
+    {
+
+
+
+
+var var_z := LV(" var_z ");
+var var_cmp := LV(" var_cmp ");
+var var_x := LV(" var_x ");
+var var_if_then := LV(" var_if_then ");
+var var_lor_lhs_false := LV(" var_lor_lhs_false ");
+var var_cmp1 := LV(" var_cmp1 ");
+var var_if_end := LV(" var_if_end ");
+var var_add := LV(" var_add ");
+var var_0 := LV(" var_0 ");
+var var_cmp2 := LV(" var_cmp2 ");
+var var_if_then3 := LV(" var_if_then3 ");
+var var_if_end4 := LV(" var_if_end4 ");
+
+var entry := Block([Ins(ALLOCA(var_z)),
+Ins(ICMP(var_cmp,slt,4,var_x,D(Int(0,IntType(4,false))))),
+Ins(BR(var_cmp,var_if_then,var_lor_lhs_false))]);
+
+var lor_lhs_false := Block([Ins(ICMP(var_cmp1,sgt,4,var_x,D(Int(2,IntType(4,false))))),
+Ins(BR(var_cmp1,var_if_then,var_if_end))]);
+
+
+
+
+        entry
+    }
+
+}
